%
% Copyright Â© 2018 Peeter Joot.  All Rights Reserved.
% Licenced as described in the file LICENSE under the root directory of this GIT repository.
%
%{
\label{chap:stressTensorAlgebraically}
Did you cry cheater because of the reliance on brute force computer assisted symbolic algebra to find the \( T(\Ba) \) relations of \cref{eqn:poyntingF:820}?
Or did you try this as a problem, and need some assistance?

If so, here is an expansion of the energy momentum tensor for vector parameters.  We start with
\begin{equation}\label{eqn:stressTensorAlgebraically:1120}
\begin{aligned}
F \Be_i
&= \lr{ \BE + I \eta \BH } \Be_i \\
&= E_i + \BE \wedge \Be_i + I \eta \lr{ H_i + \BH \wedge \Be_i }.
\end{aligned}
\end{equation}

To show that the scalar grades are related to the Poynting vector as \( \gpgradezero{T(\Be_i)} = - \BS \cdot \Be_i/ c \), we need the scalar grades of the tensor for vector parameters
\begin{equation}\label{eqn:stressTensorAlgebraically:1180}
\begin{aligned}
\frac{\epsilon}{2} \gpgradezero{ F \Be_i F^\dagger }
&=
\frac{\epsilon}{2} \gpgradezero{
   \cancel{E_i \BE}
   + I \eta \lr{ \BH \wedge \Be_i } \BE
   + \cancel{\lr{\BE \wedge \Be_i } \cdot \BE}
   + \cancel{I \eta H_i \BE}
} \\
&\quad+ \frac{\epsilon}{2} \eta
\gpgradezero{
   - \cancel{E_i I \BH}
   + \cancel{\eta \lr{ \BH \wedge \Be_i } \cdot \BH}
   - \lr{ \BE \wedge \Be_i } I \BH
   + \cancel{\eta H_i \BH}
} \\
&=
\frac{\epsilon}{2} \gpgradezero{
   I^2 \eta \lr{ \BH \cross \Be_i } \BE
   - \eta \lr{ \BE \cross \Be_i } I^2 \BH
} \\
&=
- \lr{ \BE \cross \BH } \cdot \Be_i/c,
\end{aligned}
\end{equation}
which is the Poynting relationship that was asserted.
For the vector grades we have
\begin{equation}\label{eqn:stressTensorAlgebraically:1140}
\begin{aligned}
&\gpgradeone{ F \Be_i F^\dagger } \\
&=
\gpgradeone{
\lr{
   E_i
   + I \eta \lr{ \BH \wedge \Be_i }
   + \BE \wedge \Be_i
   + I \eta H_i
}
\lr{
   \BE - I \eta \BH
}
} \\
&=
\gpgradeone{
   E_i \BE
   + \cancel{I \eta \lr{ \BH \wedge \Be_i } \BE}
   + \lr{\BE \wedge \Be_i } \cdot \BE
   + \cancel{I \eta H_i \BE}
} \\
&\qquad + \eta
\gpgradeone{
   - \cancel{E_i I \BH}
   + \eta \lr{ \BH \wedge \Be_i } \cdot \BH
   - \cancel{\lr{ \BE \wedge \Be_i } I \BH}
   + \eta H_i \BH
} \\
&=
   E_i \BE
   + \BE E_i - \BE^2 \Be_i
   + \eta^2 \BH H_i - \eta^2 \BH^2 \Be_i
   + \eta^2 H_i \BH \\
&=
   2 E_i \BE - \BE^2 \Be_i
   + \eta^2 \lr{ 2 H_i \BH - \BH^2 \Be_i }.
\end{aligned}
\end{equation}

Assembling all the results, we have
\begin{equation}\label{eqn:stressTensorAlgebraically:1160}
\gpgradeone{T(\Be_i)} \cdot \Be_j
=
\frac{\epsilon}{2}
\lr{
   2 E_i E_j - \BE^2 \delta_{ij}
   + \eta^2 \lr{ 2 H_i H_j - \BH^2 \delta_{ij} }
},
\end{equation}
which proves that \( \gpgradeone{T(\Be_i)} \cdot \Be_j = -\Theta^{ij} \) as stated in
\cref{dfn:poyntingF:1180}.
%}
